tarski/frontend/tests/fixtures/arrow-this.js
@@ -1,0 +1,13 @@
+"use strict";
+const counter = {
+  n: 0,
+  bump: function () {
+    const step = () => {
+      this.n = this.n + 1;
+      return this.n;
+    };
+    return step();
+  },
+};
+counter.bump();
+counter.bump();
