tarski/frontend/tests/fixtures/unsupported-default-param.js
@@ -1,0 +1,5 @@
+"use strict";
+function f(x = 1) {
+  return x;
+}
+f();
